StlcNormalizing.fst
@@ -1,16 +1,16 @@
 module StlcNormalizing
 
 open StlcCbvDbParSubst
-open Constructive
+open FStar.Constructive
 
 let ok = magic
 let ok_a = admit
 
-       
+
 (*** Facts about substitution and closedness *)
 val id : sub
 let id (x : var) = EVar x
-                        
+
 val subst_id : e:exp -> Lemma (subst id e = e)
 let rec subst_id e =
   match e with
@@ -19,38 +19,40 @@ let rec subst_id e =
   | ELam t e -> subst_id e
 (* by_induction_on e subst_id -- requires huge timeout (50s)! *)
 
-val update : sub -> var -> exp -> Tot sub                        
+val update : sub -> var -> exp -> Tot sub
 let update s x v y = if y = x then v else s y
 type closed (e : exp) = (forall y. not(appears_free_in y e))
 type closed2 (sigma:sub) = (forall x. sigma x <> EVar x ==> closed(sigma x))
 
 val closed_app : e1 : exp -> e2:exp -> Lemma (requires (closed (EApp e1 e2))) (ensures (closed e1 /\ closed e2))
 let closed_app e1 e2 = ()
-                    
-val subst_closed : e:exp -> 
+
+val subst_closed : e:exp ->
    Lemma (requires (closed e)) (ensures (forall sigma. subst sigma e = e))
 let rec subst_closed e =
   match e with
   | EApp e1 e2 -> closed_app e1 e2; subst_closed e1; subst_closed e2
   | ELam t1 e1 -> admit() (* needs work, or different definition of closedness *)
+  | EVar _ -> () (* TODO: really silly that this is needed, filed as #576 *)
 
 val substitution_lemma' : #g:env -> g':env -> #e:exp -> #t:typ -> sigma:sub ->
                           typing g e t ->
-                          (x:var -> t:typ{g x == Some t} -> g'':env -> Tot (typing g'' (sigma x) t)
-                                                                           (requires (sigma x <> EVar x))
-                                                                           (ensures True)) ->
+                          (x:var -> t:typ{g x == Some t} -> g'':env -> Pure (typing g'' (sigma x) t)
+                                                                            (requires (b2t (sigma x <> EVar x)))
+                                                                            (ensures (fun _ -> True))) ->
                           (x:var -> t:typ -> Lemma (requires (g x == Some t /\ sigma x == EVar x))
                                                    (ensures (g' x == Some t))) ->
                           Tot (typing g' (subst sigma e) t)
-let rec substitution_lemma' g g' e t sigma ty_g h1 h2 =
+let rec substitution_lemma' #g g' #e #t sigma ty_g h1 h2 =
   match ty_g with
   | TyVar x -> if sigma x <> EVar x then h1 x t g' else (h2 x t; TyVar x)
   | TyApp #g_ #e1 #e2 ih1 ih2 -> TyApp (substitution_lemma' g' sigma ih1 h1 (fun x t -> h2 x t)) (substitution_lemma' g' sigma ih2 h1 (fun x t -> h2 x t))
   | TyLam #g t1 #e1 #t2 ih1 ->
      TyLam t1 (substitution_lemma' (extend g' 0 t1) (subst_elam sigma) ih1 (ok()) (fun x t -> ok_a()))
 
-val invariance_env : #e:exp -> #t:typ -> g:env -> g':env -> typing g e t -> Tot (typing g' e t) (requires (forall x. is_Some (g x) ==> g x == g' x)) (ensures True)
-let rec invariance_env e t g g' ty_g =
+val invariance_env : #e:exp -> #t:typ -> g:env -> g':env -> typing g e t ->
+  Pure (typing g' e t) (requires (forall x. is_Some (g x) ==> g x == g' x)) (fun _ -> ensures True)
+let rec invariance_env #e #t g g' ty_g =
   match ty_g with
   | TyApp ty_arrow ty_arg -> TyApp (invariance_env g g' ty_arrow) (invariance_env g g' ty_arg)
   | TyLam argT ty_ext -> TyLam argT (invariance_env (extend g 0 argT) (extend g' 0 argT) ty_ext)
@@ -58,22 +60,25 @@ let rec invariance_env e t g g' ty_g =
 
 val invariance_empty : #e:exp -> #t:typ ->
   typing empty e t -> g:env -> Tot ( typing g e t )
-let invariance_empty e t ty g = invariance_env #e #t empty g ty
-                                   
+let invariance_empty #e #t ty g = invariance_env #e #t empty g ty
+
 val substitution_lemma : #g:env -> g':env -> #e:exp -> #t:typ -> sigma:sub ->
                          typing g e t ->
                          (x:var -> t:typ{g x == Some t} -> Tot (cexists (fun e -> h:(typing empty e t){sigma x == e}))) ->
                          Tot (typing g' (subst sigma e) t)
-let rec substitution_lemma g g' e t sigma ty_g h2 =                             
+let rec substitution_lemma #g g' #e #t sigma ty_g h2 =
   substitution_lemma' g' sigma ty_g (fun x t g'' -> match h2 x t with
-                                                      ExIntro s h -> let (u:unit{g x == Some t}) = ok() in
+                                                    | ExIntro s h -> let (u:unit{g x == Some t}) = ok() in
                                                                      invariance_empty h g'')
-                      (fun x t -> match h2 x t with ExIntro s h -> ())       
+                      (fun x t -> match h2 x t with | ExIntro s h -> ())
 
 
 val subst_update : x:var -> v:exp -> e:exp -> sigma:sub{closed2 sigma} ->
                    Lemma (subst_beta v (subst (subst_elam sigma) e) = subst (update (subst_elam sigma) 0 v) e)
-let rec subst_update x v e sigma = match e with
+let rec subst_update x v e sigma = admit()
+
+(* TODO: verification loops for this
+  match e with
   | EVar x -> if x > 0 then
                 (
                   if (sigma (x-1) <> EVar (x-1)) then
@@ -87,37 +92,40 @@ let rec subst_update x v e sigma = match e with
                     )
                 )
   | EApp e1 e2 -> subst_update x v e1 sigma; subst_update x v e2 sigma
-  | _ -> admit() (* fiddly *)                      
-                      
-(*** Evaluation and halting terms *)                       
-       
+  | _ -> admit() (* fiddly *)
+*)
+
+(*** Evaluation and halting terms *)
+
 kind Relation (a:Type) = a -> a -> Type
+
+(* TODO this loops, filed as #575 *)
 type multi (a:Type) (r:Relation a) : a -> a -> Type =
 | Multi_refl : x:a -> multi a r x x
 | Multi_step : x:a -> y:a -> z:a -> r x y -> multi a r y z -> multi a r x z
 type steps : exp -> exp -> Type = fun x y -> multi exp step x y
 type halts (e:exp) : Type = cexists (fun e' -> u:(steps e e'){is_value e'})
 
-                                    
+
 val value_normal : v:exp{is_value v} -> Tot (halts v)
-let value_normal v = match v with ELam _ _ -> ExIntro v (Multi_refl v)
+let value_normal v = match v with | ELam _ _ -> ExIntro v (Multi_refl v)
 
 val step_deterministic : e:exp -> e':exp -> e'':exp -> step e e' -> step e e'' -> Lemma (e' = e'')
 let rec step_deterministic e e' e'' step1 step2 =
   match step1 with
-  | SApp1 #fe1 fe2 #fe1' fstep_e1 -> 
+  | SApp1 #fe1 fe2 #fe1' fstep_e1 ->
      (match step2 with
       | SApp1 #se1 se2 #se1' sstep_e1 ->
 	     assert(fe1 == se1);
-	     step_deterministic fe1 fe1' se1' fstep_e1 sstep_e1; 
+	     step_deterministic fe1 fe1' se1' fstep_e1 sstep_e1;
 	     step_deterministic se1 fe1' se1' fstep_e1 sstep_e1
       | _ -> ()
      )
-  | SApp2 fe1 #fe2 #fe2' fstep_e2 -> 
+  | SApp2 fe1 #fe2 #fe2' fstep_e2 ->
      (match step2 with
-      | SApp2 se1 #se2 #se2' sstep_e2 -> 
+      | SApp2 se1 #se2 #se2' sstep_e2 ->
 	     assert(fe2 == se2);
-	     step_deterministic fe2 fe2' se2' fstep_e2 sstep_e2; 
+	     step_deterministic fe2 fe2' se2' fstep_e2 sstep_e2;
 	     step_deterministic se2 fe2' se2' fstep_e2 sstep_e2
       | SApp1 #se1 se2 #se1' sstep_e1 -> ()
       | _ -> ()
@@ -129,22 +137,22 @@ let rec step_deterministic e e' e'' step1 step2 =
       | SBeta argT' body' arg' -> ()
      )
 
-val step_preserves_halting : e:exp -> e':exp -> step e e' -> Tot (ciff (halts e) (halts e'))           
+val step_preserves_halting : e:exp -> e':exp -> step e e' -> Tot (ciff (halts e) (halts e'))
 let rec step_preserves_halting e e' s_e_e' =
   let p1 : (halts e -> Tot (halts e')) =
     fun (h : halts e) ->
-    match h with ExIntro v to_v ->
+    match h with | ExIntro v to_v ->
       match to_v with
       | Multi_step e1 e'' e2 s_e_e'' st_e''_v -> step_deterministic e e' e'' s_e_e' s_e_e'';
                                                  ExIntro v st_e''_v
   in let p2 : (halts e' -> Tot (halts e)) =
      fun (h : halts e') ->
-     match h with ExIntro v to_v -> ExIntro v (Multi_step e e' v s_e_e' to_v)
-  in                                          
+     match h with | ExIntro v to_v -> ExIntro v (Multi_step e e' v s_e_e' to_v)
+  in
     Conj p1 p2
 
-       
-(*** The relation red *)                                                      
+
+(*** The relation red *)
 
 (* This has a negative occurrence of R that makes Coq succumb,
 although this definition is just fine (the type decreases);
@@ -196,7 +204,7 @@ let red_halts t e h =
   match h with
   | R_arrow _ _ _ hh _ -> hh
   | R_bool _ hh -> hh
-                                                           
+
 val red_typable_empty : #t:typ -> #e:exp -> red t e -> Tot (typing empty e t)
 let red_typable_empty t e h =
   match h with
@@ -210,10 +218,10 @@ let rec step_preserves_red e e' s_e_e' t h =
   match t with
   | TArr t1 t2 ->
      (match h with
-      | R_bool t_e ht -> R_bool t_e (red_halts h) 
+      | R_bool t_e ht -> R_bool t_e (red_halts h)
       | R_arrow t1 t2 ty_e h_e f ->
 	let has_typ_e' : (typing empty e' t) = preservation s_e_e' ty_e in
-	let p : (halts e') = match (step_preserves_halting e e' s_e_e') with Conj pa pb -> pa h_e in
+	let p : (halts e') = match (step_preserves_halting e e' s_e_e') with | Conj pa pb -> pa h_e in
 	let ff : (e'':exp -> red t1 e'' -> Tot (red t2 (EApp e' e''))) =
           fun e'' red_t1_e'' -> let h' : (red t2 (EApp e e'')) = f e'' red_t1_e'' in
 				step_preserves_red (EApp e e'') (EApp e' e'') (SApp1 e'' s_e_e') t2 h'	in
@@ -224,23 +232,23 @@ let rec step_preserves_red e e' s_e_e' t h =
 	 let has_typ_e' : (typing empty e' t) = preservation s_e_e' t_e in
 	 let p : (halts e') =
 	   match (step_preserves_halting e e' s_e_e') with
-	     Conj pa pb -> pa ht in
+	   | Conj pa pb -> pa ht in
 	 R_bool has_typ_e' p )
-	       
-                            
+
+
 val steps_preserves_red : e:exp -> e':exp -> b:steps e e' -> t:typ -> red t e -> Tot (red t e') (decreases b)
-let rec steps_preserves_red e e' st_e_e' t h = 
+let rec steps_preserves_red e e' st_e_e' t h =
   match st_e_e' with
   | Multi_refl e''1 -> h
-  | Multi_step e1 e'' e'1 s_e_e'' st_e''_e' -> 
+  | Multi_step e1 e'' e'1 s_e_e'' st_e''_e' ->
      steps_preserves_red e'' e' st_e''_e' t (step_preserves_red e e'' s_e_e'' t h)
-               
-val step_preserves_red' : e:exp -> e':exp -> step e e' -> t:typ -> typing empty e t -> red t e' -> Tot (red t e) (decreases t)         
+
+val step_preserves_red' : e:exp -> e':exp -> step e e' -> t:typ -> typing empty e t -> red t e' -> Tot (red t e) (decreases t)
 let rec step_preserves_red' e e' s_e_e' t ty_t h =
    match t with
   | TArr t1 t2 ->
-     (match h with R_arrow t1 t2 ty_e h_e f ->
-       let p : (halts e) = match (step_preserves_halting e e' s_e_e') with Conj pa pb -> pb h_e in
+     (match h with | R_arrow t1 t2 ty_e h_e f ->
+       let p : (halts e) = match (step_preserves_halting e e' s_e_e') with | Conj pa pb -> pb h_e in
        let ff : (e'':exp -> red t1 e'' -> Tot (red t2 (EApp e e''))) =
          fun e'' red_t1_e'' -> let h' : (red t2 (EApp e' e'')) = f e'' red_t1_e'' in
                                let ty_e'' : (typing empty e'' t1) = red_typable_empty red_t1_e'' in
@@ -252,17 +260,17 @@ let rec step_preserves_red' e e' s_e_e' t ty_t h =
   | TBool ->
      (match h with
       | R_bool t_e ht ->
-	 let p : (halts e) = match (step_preserves_halting e e' s_e_e') with Conj pa pb -> pb ht in
+	 let p : (halts e) = match (step_preserves_halting e e' s_e_e') with | Conj pa pb -> pb ht in
 	 R_bool ty_t p
-     )                       
-                                        
-(*** The relations red2 and ered *)                       
+     )
+
+(*** The relations red2 and ered *)
 
 type red2 (g:env) (sigma:sub) =
     cand (x : var -> t : typ{g x == Some t} -> Tot (cexists (fun e -> h:(red t e){sigma x == e})))
          (x : var -> e : exp{sigma x == e /\ EVar x <> e} -> Tot (cexists (fun t -> h:(red t e){g x == Some t})))
 type ered (t : typ) (e : exp) = e':exp -> step e e' -> Tot (red t e')
-                                                           
+
 val red_subst : g:env -> e:exp -> t:typ -> sigma:sub ->
                 typing g e t ->
                 red2 g sigma ->
@@ -274,7 +282,7 @@ let red_subst g e t sigma ty_t r = substitution_lemma empty sigma ty_t
                                          ExIntro s (red_typable_empty h1))
 
 assume val typing_closed : #e:exp -> #t:typ -> typing empty e t -> Lemma (closed e)
-                                        
+
 val red2_preserves_update :
     #g:env -> #sigma:sub -> t':typ -> u:exp -> red t' u ->
     red2 g sigma -> Tot ( red2 (extend g 0 t') (update (subst_elam sigma) 0 u) )
@@ -317,7 +325,7 @@ let red2_preserves_update g sigma t' u red_u red2_g = ok()
   (*           ExIntro t' red_u *)
   (*         ) *)
   (*      ) *)
-                     
+
 val red_exp_closed : #t:typ -> e:exp{not (is_value e)} ->
                      typing empty e t ->
                      ered t e ->
@@ -333,31 +341,31 @@ val red_beta_induction : t1:typ -> t2:typ -> e:exp ->
 	       Tot (red t2 (EApp (ELam t1 e) e'))
 let rec red_beta_induction t1 t2 e ty_t2 f e' red_e' v steps_e'v =
   match steps_e'v with
-  | Multi_step same_e' e'' same_v step_e'e'' mult_e''v -> 
-     red_exp_closed #t2 (EApp (ELam t1 e) e') (TyApp (TyLam #empty t1 #e #t2 ty_t2) (red_typable_empty #t1 #e' red_e')) 
-     (fun exp_e (stp : step (EApp (ELam t1 e) e') exp_e) -> 
+  | Multi_step same_e' e'' same_v step_e'e'' mult_e''v ->
+     red_exp_closed #t2 (EApp (ELam t1 e) e') (TyApp (TyLam #empty t1 #e #t2 ty_t2) (red_typable_empty #t1 #e' red_e'))
+     (fun exp_e (stp : step (EApp (ELam t1 e) e') exp_e) ->
       ( match stp with
-	| SApp2 lambda #same_e' #same_e'' stp_e' -> 
+	| SApp2 lambda #same_e' #same_e'' stp_e' ->
 	   step_deterministic e' e'' same_e'' step_e'e'' stp_e';
-	   assert(exp_e == (EApp (ELam t1 e) e'')); 
+	   assert(exp_e == (EApp (ELam t1 e) e''));
 	   assert(multi exp step e'' v == steps e'' v);
 	   assert(same_v == v);
-	   red_beta_induction t1 t2 e ty_t2 f e'' (step_preserves_red e' e'' step_e'e'' t1 red_e') v (ok())(*mult_e''v*) 
+	   red_beta_induction t1 t2 e ty_t2 f e'' (step_preserves_red e' e'' step_e'e'' t1 red_e') v (ok())(*mult_e''v*)
 	| SBeta same_t1 same_e same_e' -> f e' red_e'
 	| _ -> ok() (* the two cases above are exhaustive... *)
       )
      )
   | Multi_refl same_e' -> step_preserves_red' (EApp (ELam t1 e) e') (subst_beta e' e) (SBeta t1 e e') t2 (TyApp (TyLam #empty t1 #e #t2 ty_t2) (red_typable_empty #t1 #e' red_e')) (f e' red_e')
-				  
+
 
 val red_beta : t1:typ -> t2:typ -> e:exp ->
                typing (extend empty 0 t1) e t2 ->
                (e' : exp -> red t1 e' -> Tot (red t2 (subst_beta e' e))) ->
                e' : exp -> red t1 e' -> Tot (red t2 (EApp (ELam t1 e) e'))
 let red_beta t1 t2 e ty_t2 f e' red_e' =
-  let ExIntro v steps_e'v = red_halts red_e' 
+  let ExIntro v steps_e'v = red_halts red_e'
   in red_beta_induction t1 t2 e ty_t2 f e' red_e' v steps_e'v
-                                                                
+
 
 val red2_closed' : #g : env -> #sigma : sub ->
                    red2 g sigma -> Lemma (closed2 sigma)
@@ -365,7 +373,7 @@ let red2_closed' g sigma red2_g = ok_a() (* logically, this is trivial
                                              but it needs at least another axiom *)
 
 (*** The main lemma and the final theorem *)
-                        
+
 val main :
       e:exp -> #t:typ -> #t':typ -> #g:env -> sigma:sub ->
       red2 g sigma ->
@@ -384,11 +392,11 @@ let rec main e t t' g sigma red2_g ty_t =
      let b : typing empty (subst sigma e) (TArr t1 t2) = (red_subst g e t sigma  ty_t red2_g) in
      let ex : halts (subst sigma e) = ExIntro (subst sigma e) (Multi_refl (subst sigma e)) in
      let e1' = (subst (subst_elam sigma) e1) in
-     let f : (s: exp -> red t1 s -> Tot ( red t2 (EApp (subst sigma e) s) )) = 
+     let f : (s: exp -> red t1 s -> Tot ( red t2 (EApp (subst sigma e) s) )) =
        (fun s h1 ->
         assert (e == ELam t1 e1);
         assert (subst sigma e == ELam t1 (subst (subst_elam sigma) e1));
-        let p : (typing (extend empty 0 t1) (e1') t2) = (match b with TyLam bla h4 -> h4) in
+        let p : (typing (extend empty 0 t1) (e1') t2) = (match b with | TyLam bla h4 -> h4) in
         let f : (u:exp -> red t1 u -> Tot (red t2 (subst_beta u e1'))) = fun u red_u ->
           red2_closed' red2_g;
           subst_update 0 u e1 sigma;
@@ -403,7 +411,7 @@ let rec main e t t' g sigma red2_g ty_t =
 
 (* This may help to prove the following fact *)
 assume val exfalso_quodlibet : unit -> Tot 'a (requires (False)) (ensures True)
-                                         
+
 val red2_id_empty : red2 empty id
 let red2_id_empty = Conj (fun x e -> exfalso_quodlibet()) (fun x t -> exfalso_quodlibet())
 
